Affine/Substitution.lean
@@ -32,6 +32,74 @@ def substₑ (e₁ : Lambda) (x : ℕ) (e₂ : Lambda) : Lambda :=
       .abs x' (e₁.substₑ x e₂)
 termination_by e₁.depth
 
+theorem substᵥ_free {e : Lambda} : (e.substᵥ x y).free = e.free \ {x} ∪ {y} := by sorry
+
+theorem substₑ_free {e₁ e₂ : Lambda} : (substₑ e₁ x e₂).free ⊆ e₁.free \ {x} ∪ e₂.free := by
+  match e₁ with
+  | .var x' =>
+    simp only [free, substₑ, apply_ite]
+    by_cases hx : x = x'
+    · simp only [if_pos hx, Finset.subset_union_right]
+    · simp only [if_neg hx, Finset.subset_union_left,
+        Finset.sdiff_singleton_eq_self (Finset.mem_singleton.not.mpr hx)]
+  | .abs x' e₁ =>
+    simp only [free, substₑ]
+    wlog hx : x ≠ x'
+    · simp only [not_not] at hx
+      simp only [if_pos (Or.inl hx), free, hx, Finset.sdiff_sdiff_left', Finset.inter_self,
+        Finset.subset_union_left]
+    wlog hxfree : x ∈ e₁.free
+    · simp only [if_pos (Or.inr hxfree), free]
+      intro v hv
+      apply Finset.mem_union_left
+      simp only [Finset.mem_sdiff, Finset.mem_singleton] at hv
+      simp only [Finset.mem_sdiff, Finset.mem_singleton]
+      have hvx : v ≠ x := by intro hvx; rw [hvx] at hv; exact hxfree hv.left
+      exact ⟨hv, hvx⟩
+    rw [if_neg]
+    by_cases hx' : x' ∈ e₂.free
+    · simp only [if_pos hx', free]
+      have hinc := substₑ_free (e₁ := e₁.substᵥ x' e₂.free.fresh) (e₂ := e₂) (x := x)
+      rw [substᵥ_free] at hinc
+      intro v hv
+      simp only [Finset.mem_sdiff, Finset.mem_singleton] at hv
+      have ⟨hv₁, hv₂⟩ := hv
+      have hv' := hinc hv₁
+      simp only [Finset.mem_union, Finset.mem_sdiff, Finset.mem_singleton, hv₂, or_false] at hv'
+      simp only [Finset.mem_union, Finset.mem_sdiff, Finset.mem_singleton]
+      exact hv'
+    · simp only [if_neg hx', free]
+      have hinc := substₑ_free (e₁ := e₁) (e₂ := e₂) (x := x)
+      intro v hv
+      simp only [Finset.mem_sdiff, Finset.mem_singleton] at hv
+      have ⟨hv₁, hv₂⟩ := hv
+      have hv' := hinc hv₁
+      simp only [Finset.mem_union, Finset.mem_sdiff, Finset.mem_singleton, hv₂, or_false] at hv'
+      simp only [Finset.mem_union, Finset.mem_sdiff, Finset.mem_singleton]
+      apply Or.elim hv'
+      · intro hv; exact Or.inl ⟨⟨hv.left, hv₂⟩, hv.right⟩
+      · exact Or.inr
+
+    case hnc => simp only [not_or, not_not, hx, hxfree, not_false_eq_true, true_and]
+  | .app a₁ a₂ =>
+    simp only [free, substₑ]
+    intro v hv
+    simp only [Finset.mem_union, Finset.mem_sdiff, Finset.mem_singleton] at hv
+    apply Or.elim hv
+    · intro hv₁
+      have hv₁ := substₑ_free hv₁
+      simp only [Finset.mem_union, Finset.mem_sdiff, Finset.mem_singleton] at hv₁
+      simp only [Finset.mem_union, Finset.mem_sdiff, Finset.mem_singleton]
+      exact Or.elim hv₁ (fun hv' => Or.inl ⟨Or.inl hv'.left, hv'.right⟩) Or.inr
+    · intro hv₂
+      have hv₂ := substₑ_free hv₂
+      simp only [Finset.mem_union, Finset.mem_sdiff, Finset.mem_singleton] at hv₂
+      simp only [Finset.mem_union, Finset.mem_sdiff, Finset.mem_singleton]
+      apply Or.elim hv₂ (fun hv' => Or.inl ⟨Or.inr hv'.left, hv'.right⟩) Or.inr
+
+termination_by e₁.depth
+
+
 theorem substᵥ_count_β {e : Lambda} : (e.substᵥ x y).count_β = e.count_β := by sorry
 
 theorem substₑ_count {e₁ e₂ : Lambda} :
@@ -54,42 +122,40 @@ theorem substₑ_count {e₁ e₂ : Lambda} :
   --   simp only [substₑ]
   --   sorry
 
-theorem substₑ_free {e₁ e₂ : Lambda} : (substₑ e₁ x e₂).free ⊆ e₁.free \ {x'} ∪ e₂.free := by
-  sorry
-
 theorem is_affine_substₑ {e₁ e₂ : Lambda} (he₁ : e₁.is_affine) (he₂ : e₂.is_affine) (x : ℕ) :
     (e₁.substₑ x e₂).is_affine := by
   sorry
 
-theorem substₑ_count_β {e₁ e₂ : Lambda} :
+theorem substₑ_count_β {e₁ e₂ : Lambda} (h₁ : e₁.is_affine) (h₂ : e₂.is_affine) :
     (e₁.substₑ x e₂).count_β < 1 + e₁.count_β + e₂.count_β := by
-  match e₁ with
-  | .var x' =>
-    have h₁ : e₂.count_β < 1 + e₂.count_β := lt_one_add _
-    have h₂ : 0 < 1 + e₂.count_β := by simp only [add_pos_iff, zero_lt_one, true_or]
-    simp only [substₑ, count_β, add_zero, apply_ite, ite_lt h₁ h₂]
+  sorry
+  -- match e₁ with
+  -- | .var x' =>
+  --   have h₁ : e₂.count_β < 1 + e₂.count_β := lt_one_add _
+  --   have h₂ : 0 < 1 + e₂.count_β := by simp only [add_pos_iff, zero_lt_one, true_or]
+  --   simp only [substₑ, count_β, add_zero, apply_ite, ite_lt h₁ h₂]
 
-  | .abs x' e₁ =>
-    simp only [substₑ, count_β, apply_ite count_β]
-    wlog hx₁ : x ∈ e₁.free
-    · simp only [if_pos (Or.inr hx₁), add_assoc, Nat.lt_one_add_iff.mpr, le_add_iff_nonneg_right,
-        zero_le]
-    wlog hxeq : x ≠ x'
-    · simp only [if_pos (Or.inl (not_not.mp hxeq)), add_assoc, Nat.lt_one_add_iff.mpr,
-        le_add_iff_nonneg_right, zero_le]
-    rw [if_neg]
-    by_cases hx' : x' ∈ e₂.free
-    · rw [if_pos hx']
-      have hinc := substₑ_count_β (e₁ := e₁.substᵥ x' e₂.free.fresh) (e₂ := e₂) (x := x)
-      simp [substᵥ_count_β] at hinc
-      exact hinc
-    · simp only [if_neg hx', substₑ_count_β (e₁ := e₁)]
-    simp only [not_or, not_not, hx₁, hxeq, not_false_eq_true, true_and]
+  -- | .abs x' e₁ =>
+  --   simp only [substₑ, count_β, apply_ite count_β]
+  --   wlog hx₁ : x ∈ e₁.free
+  --   · simp only [if_pos (Or.inr hx₁), add_assoc, Nat.lt_one_add_iff.mpr, le_add_iff_nonneg_right,
+  --       zero_le]
+  --   wlog hxeq : x ≠ x'
+  --   · simp only [if_pos (Or.inl (not_not.mp hxeq)), add_assoc, Nat.lt_one_add_iff.mpr,
+  --       le_add_iff_nonneg_right, zero_le]
+  --   rw [if_neg]
+  --   by_cases hx' : x' ∈ e₂.free
+  --   · rw [if_pos hx']
+  --     have hinc := substₑ_count_β (e₁ := e₁.substᵥ x' e₂.free.fresh) (e₂ := e₂) (x := x)
+  --     simp [substᵥ_count_β] at hinc
+  --     exact hinc
+  --   · simp only [if_neg hx', substₑ_count_β (e₁ := e₁)]
+  --   simp only [not_or, not_not, hx₁, hxeq, not_false_eq_true, true_and]
 
-  | .app a₁ a₂ =>
-    simp only [substₑ, count_β]
-    have x := count_β_of_app (e₁ := substₑ a₁ x e₂) (e₂ := substₑ a₂ x e₂)
+  -- | .app a₁ a₂ =>
+  --   simp only [substₑ, count_β]
+  --   have x := count_β_of_app (e₁ := substₑ a₁ x e₂) (e₂ := substₑ a₂ x e₂)
 
-termination_by e₁.depth
+-- termination_by e₁.depth
 
 end Lambda
